Infrastructure.v
@@ -1,0 +1,87 @@
+Require Export Fsub.Definitions.
+
+Fixpoint fv_tt (T : typ) {struct T} : atoms :=
+  match T with
+  | typ_top => {}
+  | typ_bvar J => {}
+  | typ_fvar X => {{ X }}
+  | typ_arrow T1 T2 => (fv_tt T1) `union` (fv_tt T2)
+  | typ_all T1 T2 => (fv_tt T1) `union` (fv_tt T2)
+  end.
+
+Fixpoint subst_tt (Z : atom) (U : typ) (T : typ) {struct T} : typ :=
+  match T with
+  | typ_top => typ_top
+  | typ_bvar J => typ_bvar J
+  | typ_fvar X => if X == Z then U else T
+  | typ_arrow T1 T2 => typ_arrow (subst_tt Z U T1) (subst_tt Z U T2)
+  | typ_all T1 T2 => typ_all (subst_tt Z U T1) (subst_tt Z U T2)
+  end.
+
+Ltac gather_atoms ::=
+  let A := gather_atoms_with (fun x : atoms => x) in
+  let B := gather_atoms_with (fun x : atom => singleton x) in
+  let C := gather_atoms_with (fun x : typ => fv_tt x) in
+  let D := gather_atoms_with (fun x : env => dom x) in
+  constr : (A `union` B `union` C `union` D).
+
+Lemma open_tt_rec_type_aux : forall T j V i U,
+  i <> j ->
+  open_tt_rec j V T = open_tt_rec i U (open_tt_rec j V T) ->
+  T = open_tt_rec i U T.
+Proof with congruence || eauto.
+  induction T; intros j V i U Neq H; simpl in *; inversion H; f_equal...
+  - destruct (j === n)... destruct (i === n)...
+Qed.
+
+Lemma open_tt_rec_type : forall T U k,
+  type T ->
+  T = open_tt_rec k U T.
+Proof with auto.
+  intros T U k Htyp. revert k.
+  induction Htyp; intros k; simpl; f_equal...
+  - unfold open_tt in *.
+    pick fresh X.
+    apply (open_tt_rec_type_aux T2 0 (typ_fvar X))...
+Qed.
+
+Lemma subst_tt_open_tt_rec : forall T1 T2 X P k,
+  type P ->
+  subst_tt X P (open_tt_rec k T2 T1) =
+    open_tt_rec k (subst_tt X P T2) (subst_tt X P T1).
+Proof with auto.
+  intros T1 T2 X P k WP. revert k.
+  induction T1; intros k; simpl; f_equal...
+  - destruct (k === n); subst...
+  - destruct (a == X); subst... apply open_tt_rec_type...
+Qed.
+
+Lemma subst_tt_open_tt_var : forall (X Y:atom) P T,
+  Y <> X ->
+  type P ->
+  open_tt (subst_tt X P T) Y = subst_tt X P (open_tt T Y).
+Proof with congruence || auto.
+  intros X Y P T Neq Wu.
+  unfold open_tt.
+  rewrite subst_tt_open_tt_rec...
+  simpl.
+  destruct (Y == X)...
+Qed.
+
+Lemma subst_tt_intro_rec : forall X T2 U k,
+  X `notin` fv_tt T2 ->
+  open_tt_rec k U T2 = subst_tt X U (open_tt_rec k (typ_fvar X) T2).
+Proof with congruence || auto.
+  induction T2; intros U k Fr; simpl in *; f_equal...
+  - destruct (k === n)... simpl. destruct (X == X)...
+  - destruct (a == X)... contradict Fr; fsetdec.
+Qed.
+
+Lemma subst_tt_intro : forall X T2 U,
+  X `notin` fv_tt T2 ->
+  open_tt T2 U = subst_tt X U (open_tt T2 X).
+Proof with auto.
+  intros.
+  unfold open_tt.
+  apply subst_tt_intro_rec...
+Qed.
