Lemmas.v
@@ -1,0 +1,207 @@
+Require Export Fsub.Infrastructure.
+
+(* wf_env *)
+
+Lemma wf_env_tailing : forall F E,
+  wf_env (F ++ E) ->
+  wf_env E.
+Proof with auto.
+  intros.
+  induction F...
+  apply IHF.
+  inversion H...
+Qed.
+
+(* uniq *)
+
+Lemma uniq_from_wf_env : forall E,
+  wf_env E ->
+  uniq E.
+Proof with auto.
+  intros; induction H...
+Qed.
+
+Hint Extern 1 (uniq ?E) => apply uniq_from_wf_env; auto : core.
+
+(* type *)
+
+Lemma type_from_wf_typ : forall E T,
+  wf_typ E T -> type T.
+Proof with eauto.
+  intros; induction H...
+Qed.
+
+Lemma type_from_wf_typ' : forall E T,
+  wf_typ' E T -> type T.
+Proof with auto.
+  intros.
+  induction H...
+  apply type_all with (L := L)...
+  apply type_from_wf_typ with (E := E)...
+Qed.
+
+Hint Extern 1 (type ?T) =>
+  match goal with
+  | H: wf_typ ?E T |- _ => apply (type_from_wf_typ E); auto
+  | H: sub ?E T _ |- _ => apply (type_from_wf_typ' E); auto
+  | H: sub ?E _ T |- _ => apply (type_from_wf_typ' E); auto
+  end : core.
+
+(* wf_typ <-> wf_typ' *)
+
+Lemma wf_typ'_from_wf_typ : forall E T,
+  wf_typ E T ->
+  wf_typ' E T.
+Proof with eauto.
+  intros; induction H...
+Qed.
+
+Hint Resolve wf_typ'_from_wf_typ : core.
+
+Hint Extern 1 (wf_typ' ?E ?T) =>
+  match goal with
+  | H: wf_typ E T |- _ => apply (proj2 (proj2 (wf_typ'_from_wf_typ E T H)))
+  end : core.
+
+(* wf_typ *)
+
+Lemma wf_typ_weakening : forall T E F G,
+  wf_typ (G ++ E) T ->
+  uniq (G ++ F ++ E) ->
+  wf_typ (G ++ F ++ E) T.
+Proof with simpl_env; eauto.
+  intros.
+  remember (G ++ E) as F'.
+  generalize dependent G.
+  induction H; intros; subst...
+  pick fresh Y and apply wf_typ_all...
+  rewrite_env ((Y ~ T1 ++ G) ++ F ++ E).
+  apply H1...
+Qed.
+
+Lemma wf_typ_weaken_head : forall T E F,
+  wf_typ E T ->
+  uniq (F ++ E) ->
+  wf_typ (F ++ E) T.
+Proof.
+  intros.
+  rewrite_env (nil ++ F ++ E).
+  auto using wf_typ_weakening.
+Qed.
+
+Lemma wf_typ_from_binds : forall X U E,
+  wf_env E ->
+  binds X U E ->
+  wf_typ E U.
+Proof with auto.
+  intros.
+  induction H.
+  - inversion H0.
+  - analyze_binds H0; rewrite_env (X0 ~ T ++ E);
+      apply wf_typ_weaken_head...
+Qed.
+
+Lemma wf_typ_subst_tt : forall F Q E Z P T,
+  wf_typ (F ++ Z ~ Q ++ E) T ->
+  wf_typ E P ->
+  uniq (map (subst_tt Z P) F ++ E) ->
+  wf_typ (map (subst_tt Z P) F ++ E) (subst_tt Z P T).
+Proof with simpl_env; eauto.
+  intros F Q E Z P T WT WP.
+  remember (F ++ Z ~ Q ++ E) as G.
+  generalize dependent F.
+  induction WT; intros F EQ Ok; subst; simpl subst_tt...
+  - destruct (X == Z); subst...
+    + rewrite_env (map (subst_tt Z P) F ++ E).
+      apply wf_typ_weaken_head; auto.
+    + analyze_binds H...
+  - pick fresh Y and apply wf_typ_all...
+    rewrite subst_tt_open_tt_var...
+    rewrite_env (map (subst_tt Z P) (Y ~ T1 ++ F) ++ E).
+    apply H0...
+Qed.
+
+Lemma wf_typ_from_wf_env : forall F X U E,
+  wf_env (F ++ X ~ U ++ E) ->
+  wf_typ E U.
+Proof with simpl_env; auto.
+  intros.
+  induction F.
+  - inversion H...
+  - apply IHF; inversion H...
+Qed.
+
+Hint Extern 3 (wf_typ ?E ?T) =>
+  match goal with
+  | H: wf_typ' E (typ_all T _) |- _ => inversion H; auto
+  end : core.
+
+(* wf_typ' *)
+
+Lemma wf_typ'_weakening : forall T E F G,
+  wf_typ' (G ++ E) T ->
+  uniq (G ++ F ++ E) ->
+  wf_typ' (G ++ F ++ E) T.
+Proof with simpl_env; eauto.
+  intros.
+  remember (G ++ E) as F'.
+  generalize dependent G.
+  induction H; intros; subst...
+  pick fresh Y and apply wf_typ'_all...
+  - apply wf_typ_weakening...
+  - rewrite_env ((Y ~ T1 ++ G) ++ F ++ E).
+    apply H1...
+Qed.
+
+Lemma wf_typ'_weaken_head : forall T E F,
+  wf_typ' E T ->
+  uniq (F ++ E) ->
+  wf_typ' (F ++ E) T.
+Proof.
+  intros.
+  rewrite_env (nil ++ F++ E).
+  auto using wf_typ'_weakening.
+Qed.
+
+Lemma wf_typ'_subst_tt : forall F Q E Z P T,
+  wf_typ' (F ++ Z ~ Q ++ E) T ->
+  wf_typ E P ->
+  uniq (map (subst_tt Z P) F ++ E) ->
+  wf_typ' (map (subst_tt Z P) F ++ E) (subst_tt Z P T).
+Proof with simpl_env; eauto.
+  intros F Q E Z P T WT WP.
+  remember (F ++ Z ~ Q ++ E) as G.
+  generalize dependent F.
+  induction WT; intros F EQ Ok; subst; simpl subst_tt...
+  - destruct (X == Z); subst...
+    + rewrite_env (map (subst_tt Z P) F ++ E).
+      apply wf_typ'_weaken_head...
+    + analyze_binds H...
+  - pick fresh Y and apply wf_typ'_all...
+    + eapply wf_typ_subst_tt...
+    + rewrite subst_tt_open_tt_var...
+      rewrite_env (map (subst_tt Z P) (Y ~ T1 ++ F) ++ E).
+      apply H1...
+Qed.
+
+Lemma wf_typ'_open : forall E U T1 T2,
+  wf_env E ->
+  wf_typ' E (typ_all T1 T2) ->
+  wf_typ E U ->
+  wf_typ' E (open_tt T2 U).
+Proof with eauto.
+  intros.
+  inversion H0; subst.
+  pick fresh Y.
+  rewrite (subst_tt_intro Y)...
+  rewrite_env (map (subst_tt Y U) nil ++ E).
+  eapply wf_typ'_subst_tt...
+Qed.
+
+Hint Extern 3 (wf_typ' ?E ?T) =>
+  match goal with
+  | H: wf_typ' E (typ_arrow T _) |- _ => inversion H; auto
+  | H: wf_typ' E (typ_arrow _ T) |- _ => inversion H; auto
+  | H: wf_typ' E (typ_all T _) |- _ => inversion H; auto
+  | H: wf_typ' E (typ_all _ T) |- _ => inversion H; auto
+  end : core.
