Theorems.v
@@ -1,35 +1,4 @@
-Require Export Fsub.Definitions.
-
-Lemma wf_typ'_from_wf_typ : forall E T,
-  wf_typ E T ->
-  wf_typ' E T.
-Proof.
-  intros.
-  induction H; eauto.
-Qed.
-
-Hint Resolve wf_typ'_from_wf_typ : core.
-
-Hint Extern 1 (wf_typ' ?E ?T) =>
-  match goal with
-  | H: wf_typ E T |- _ => apply (proj2 (proj2 (wf_typ'_from_wf_typ E T H)))
-  end : core.
-
-Lemma wf_typ_from_wf_typ' : forall E (X : atom),
-  wf_env E ->
-  wf_typ' E X ->
-  wf_typ E X.
-Proof.
-  intros.
-  inversion H0; subst; eauto.
-Qed.
-
-Hint Resolve wf_typ_from_wf_typ' : core.
-
-Hint Extern 1 (wf_typ ?E ?T) =>
-  match goal with
-  | H: wf_typ' E T |- _ => apply (proj2 (proj2 (wf_typ_from_wf_typ' E T H)))
-  end : core.
+Require Export Fsub.Lemmas.
 
 (* Reflexivity *)
 
@@ -37,213 +6,24 @@ Theorem sub_reflexivity_aux : forall E T,
   wf_env E ->
   wf_typ E T ->
   sub E T T.
-Proof.
+Proof with eauto.
   intros.
-  induction H0; eauto.
-  pick fresh Y and apply sub_all; auto.
+  induction H0...
+  pick fresh Y and apply sub_all...
 Qed.
 
 Theorem sub_reflexivity : forall E T,
   wf_env E ->
   wf_typ' E T ->
   sub E T T.
-Proof.
+Proof with eauto.
   intros.
-  induction H0; eauto.
-  pick fresh Y and apply sub_all; auto.
-  apply sub_reflexivity_aux; auto.
+  induction H0...
+  pick fresh Y and apply sub_all...
+  apply sub_reflexivity_aux...
 Qed.
 
 (* Transitivity *)
-
-Lemma wf_typ_weakening : forall T E F G,
-  wf_typ (G ++ E) T ->
-  uniq (G ++ F ++ E) ->
-  wf_typ (G ++ F ++ E) T.
-Proof.
-  intros.
-  remember (G ++ E) as F'.
-  generalize dependent G.
-  induction H; intros; subst; eauto.
-  pick fresh Y and apply wf_typ_all; auto.
-  rewrite_env ((Y ~ T1 ++ G) ++ F ++ E).
-  apply H1; auto.
-  simpl_env.
-  auto.
-Qed.
-
-Lemma wf_typ'_weakening : forall T E F G,
-  wf_typ' (G ++ E) T ->
-  uniq (G ++ F ++ E) ->
-  wf_typ' (G ++ F ++ E) T.
-Proof.
-  intros.
-  remember (G ++ E) as F'.
-  generalize dependent G.
-  induction H; intros; subst; eauto.
-  pick fresh Y and apply wf_typ'_all; auto.
-  - apply wf_typ_weakening; auto.
-  - rewrite_env ((Y ~ T1 ++ G) ++ F ++ E).
-    apply H1; auto.
-    simpl_env.
-    auto.
-Qed.
-
-Lemma uniq_from_wf_env : forall E,
-  wf_env E ->
-  uniq E.
-Proof.
-  intros E H; induction H; auto.
-Qed.
-
-Lemma wf_typ_from_binds_typ : forall X U E,
-  wf_env E ->
-  binds X U E ->
-  wf_typ E U.
-Proof.
-  intros.
-  induction H.
-  - inversion H0.
-  - analyze_binds H0; rewrite_env (nil ++ X0 ~ T ++ E);
-      apply wf_typ_weakening; auto;
-      simpl_env;
-      apply uniq_from_wf_env; auto.
-Qed.
-
-Lemma type_from_wf_typ : forall E T,
-  wf_typ E T -> type T.
-Proof.
-  intros.
-  induction H; eauto.
-Qed.
-
-Lemma type_from_wf_typ' : forall E T,
-  wf_typ' E T -> type T.
-Proof.
-  intros.
-  induction H; auto.
-  apply type_all with (L := L); auto.
-  apply type_from_wf_typ with (E := E); auto.
-Qed.
-
-Lemma subst_tt_intro_rec : forall X T2 U k,
-  X `notin` fv_tt T2 ->
-  open_tt_rec k U T2 = subst_tt X U (open_tt_rec k (typ_fvar X) T2).
-Proof with congruence || auto.
-  induction T2; intros U k Fr; simpl in *; f_equal...
-  - destruct (k === n)... simpl. destruct (X == X)...
-  - destruct (a == X)... contradict Fr; fsetdec.
-Qed.
-
-Lemma subst_tt_intro : forall X T2 U,
-  X `notin` fv_tt T2 ->
-  open_tt T2 U = subst_tt X U (open_tt T2 X).
-Proof with auto.
-  intros.
-  unfold open_tt.
-  apply subst_tt_intro_rec...
-Qed.
-
-Lemma open_tt_rec_type_aux : forall T j V i U,
-  i <> j ->
-  open_tt_rec j V T = open_tt_rec i U (open_tt_rec j V T) ->
-  T = open_tt_rec i U T.
-Proof with congruence || eauto.
-  induction T; intros j V i U Neq H; simpl in *; inversion H; f_equal...
-  - destruct (j === n)... destruct (i === n)...
-Qed.
-
-Lemma open_tt_rec_type : forall T U k,
-  type T ->
-  T = open_tt_rec k U T.
-Proof with auto.
-  intros T U k Htyp. revert k.
-  induction Htyp; intros k; simpl; f_equal...
-  - unfold open_tt in *.
-    pick fresh X.
-    apply (open_tt_rec_type_aux T2 0 (typ_fvar X))...
-Qed.
-
-Lemma subst_tt_open_tt_rec : forall T1 T2 X P k,
-  type P ->
-  subst_tt X P (open_tt_rec k T2 T1) =
-    open_tt_rec k (subst_tt X P T2) (subst_tt X P T1).
-Proof with auto.
-  intros T1 T2 X P k WP. revert k.
-  induction T1; intros k; simpl; f_equal...
-  - destruct (k === n); subst...
-  - destruct (a == X); subst... apply open_tt_rec_type...
-Qed.
-
-Lemma subst_tt_open_tt_var : forall (X Y:atom) P T,
-  Y <> X ->
-  type P ->
-  open_tt (subst_tt X P T) Y = subst_tt X P (open_tt T Y).
-Proof with congruence || auto.
-  intros X Y P T Neq Wu.
-  unfold open_tt.
-  rewrite subst_tt_open_tt_rec...
-  simpl.
-  destruct (Y == X)...
-Qed.
-
-Lemma wf_typ_subst_tt : forall F Q E Z P T,
-  wf_typ (F ++ Z ~ Q ++ E) T ->
-  wf_typ E P ->
-  uniq (map (subst_tt Z P) F ++ E) ->
-  wf_typ (map (subst_tt Z P) F ++ E) (subst_tt Z P T).
-Proof with simpl_env; eauto using type_from_wf_typ'.
-  intros F Q E Z P T WT WP.
-  remember (F ++ Z ~ Q ++ E) as G.
-  generalize dependent F.
-  induction WT; intros F EQ Ok; subst; simpl subst_tt...
-  - destruct (X == Z); subst...
-    + rewrite_env (nil ++ map (subst_tt Z P) F ++ E).
-      apply wf_typ_weakening; auto.
-    + analyze_binds H...
-  - pick fresh Y and apply wf_typ_all...
-    rewrite subst_tt_open_tt_var...
-    rewrite_env (map (subst_tt Z P) (Y ~ T1 ++ F) ++ E).
-    apply H0...
-Qed.
-
-
-Lemma wf_typ'_subst_tt : forall F Q E Z P T,
-  wf_typ' (F ++ Z ~ Q ++ E) T ->
-  wf_typ E P ->
-  uniq (map (subst_tt Z P) F ++ E) ->
-  wf_typ' (map (subst_tt Z P) F ++ E) (subst_tt Z P T).
-Proof with simpl_env; eauto using type_from_wf_typ'.
-  intros F Q E Z P T WT WP.
-  remember (F ++ Z ~ Q ++ E) as G.
-  generalize dependent F.
-  induction WT; intros F EQ Ok; subst; simpl subst_tt...
-  - destruct (X == Z); subst...
-    + rewrite_env (nil ++ map (subst_tt Z P) F ++ E).
-      apply wf_typ'_weakening; auto.
-    + analyze_binds H...
-  - pick fresh Y and apply wf_typ'_all...
-    + eapply wf_typ_subst_tt; eauto.
-    + rewrite subst_tt_open_tt_var...
-      rewrite_env (map (subst_tt Z P) (Y ~ T1 ++ F) ++ E).
-      apply H1...
-Qed.
-
-Lemma wf_typ'_open : forall E U T1 T2,
-  wf_env E ->
-  wf_typ' E (typ_all T1 T2) ->
-  wf_typ E U ->
-  wf_typ' E (open_tt T2 U).
-Proof.
-  intros.
-  inversion H0; subst.
-  pick fresh Y.
-  rewrite (subst_tt_intro Y); auto.
-  rewrite_env (map (subst_tt Y U) nil ++ E).
-  eapply wf_typ'_subst_tt; eauto.
-  simpl_env.
-  apply uniq_from_wf_env; auto.
-Qed.
 
 Lemma sub_weakening : forall E F G S T,
   wf_env (G ++ E) ->
@@ -251,75 +31,20 @@ Lemma sub_weakening : forall E F G S T,
   sub (G ++ E) S T ->
   wf_env (G ++ F ++ E) ->
   sub (G ++ F ++ E) S T.
-Proof.
+Proof with simpl_env; eauto using wf_typ_weakening, wf_typ'_weaken_head, uniq_from_wf_env.
   intros E F G S T HwfGE HwfGES HwfGET SsubT HwfGFE.
   remember (G ++ E) as H.
   generalize dependent G.
-  induction SsubT; intros G Heq HwfGFE; subst; auto.
-  - apply sub_var with (U := U); auto.
-    apply IHSsubT; auto.
+  induction SsubT; intros G Heq HwfGFE; subst...
+  - apply sub_var with (U := U)...
+    apply IHSsubT...
     apply wf_typ'_from_wf_typ.
-    apply wf_typ_from_binds_typ with (X := X); auto.
-  - apply sub_arrow; auto.
-    + apply IHSsubT1; auto.
-      * inversion HwfGET; auto.
-      * inversion HwfGES; auto.
-    + apply IHSsubT2; auto.
-      * inversion HwfGES; auto.
-      * inversion HwfGET; auto.
+    apply wf_typ_from_binds with (X := X)...
   - pick fresh Y and apply sub_all.
-    + apply IHSsubT; auto.
-      * inversion HwfGET; auto.
-      * inversion HwfGES; auto.
+    + apply IHSsubT...
     + rewrite_env ((Y ~ T1 ++ G) ++ F ++ E).
-      apply H0; auto.
-      * apply wf_env_sub; auto.
-        inversion HwfGET; auto.
-      * apply wf_typ'_open with (T1 := S1); auto.
-        -- apply wf_env_sub; auto.
-           inversion HwfGET; auto.
-        -- rewrite_env (nil ++ Y ~ T1 ++ (G ++ E)).
-           apply wf_typ'_weakening; simpl_env; auto.
-           apply uniq_from_wf_env.
-           apply wf_env_sub; auto.
-           inversion HwfGET; auto.
-        -- apply wf_typ_var with (U := T1); auto.
-      * apply wf_typ'_open with (T1 := T1); auto.
-        -- apply wf_env_sub; auto.
-           inversion HwfGET; auto.
-        -- rewrite_env (nil ++ Y ~ T1 ++ (G ++ E)).
-           apply wf_typ'_weakening; simpl_env; auto.
-           apply uniq_from_wf_env.
-           apply wf_env_sub; auto.
-           inversion HwfGET; auto.
-        -- apply wf_typ_var with (U := T1); auto.
-      * simpl_env.
-        apply wf_env_sub; auto.
-        apply wf_typ_weakening; auto.
-        -- inversion HwfGET; auto.
-        -- apply uniq_from_wf_env; auto.
+      apply H0; try eapply wf_typ'_open...
 Qed.
-
-Lemma wf_env_tailing : forall F E,
-  wf_env (F ++ E) ->
-  wf_env E.
-Proof.
-  intros.
-  induction F; auto.
-  apply IHF.
-  inversion H; auto.
-Qed.
-
-Lemma wf_typ_from_bind : forall F X U E,
-  wf_env (F ++ X ~ U ++ E) ->
-  wf_typ E U.
-Proof.
-  intros.
-  induction F; auto; simpl_env in *.
-  - inversion H; auto.
-  - apply IHF.
-    inversion H; auto.
-Qed.    
 
 Lemma sub_narrowing_aux : forall Q F E Z P S T,
   wf_env (F ++ Z ~ Q ++ E) -> wf_env (F ++ Z ~ P ++ E) ->
@@ -329,112 +54,50 @@ Lemma sub_narrowing_aux : forall Q F E Z P S T,
   sub (F ++ Z ~ Q ++ E) S T ->
   sub E P Q ->
   sub (F ++ Z ~ P ++ E) S T.
-Proof.
+Proof with simpl_env; eauto using wf_typ'_weaken_head.
   intros Q F E Z P S T HwfEq HwfEp HwfEqS HwfEqT HwfEpS HwfEpT Htrans SsubT PsubQ.
   remember (F ++ Z ~ Q ++ E) as G.
   generalize dependent F.
   induction SsubT; auto; intros F Heq HwfEp HwfEpS HwfEpT; subst.
   (* NVar *)
   - destruct (X == Z); subst.
-    + apply sub_var with (U := P); auto.
-      apply Htrans; auto.
+    + apply sub_var with (U := P)...
+      apply Htrans...
       (* wf_typ' E Q *)
-      * rewrite_env (nil ++ (F ++ Z ~ P) ++ E).
-        apply wf_typ'_weakening; simpl_env; auto.
-        -- apply wf_typ'_from_wf_typ.
-           apply wf_typ_from_bind with (F := F) (X := Z); auto.
-        -- apply uniq_from_wf_env; auto.
+      * rewrite_env ((F ++ Z ~ P) ++ E).
+        apply wf_typ'_weaken_head...
+        apply wf_typ'_from_wf_typ.
+        apply wf_typ_from_wf_env with (F := F) (X := Z)...
       (* wf_typ' E S *)
-      * rewrite_env (nil ++ (F ++ Z ~ P) ++ E).
-        apply wf_typ'_weakening; simpl_env; auto.
-        -- apply wf_typ'_from_wf_typ.
-           apply wf_typ_from_bind with (F := F) (X := Z); auto.
-        -- apply uniq_from_wf_env; auto.
+      * rewrite_env ((F ++ Z ~ P) ++ E).
+        apply wf_typ'_weaken_head...
+        apply wf_typ'_from_wf_typ.
+        apply wf_typ_from_wf_env with (F := F) (X := Z)...
       (* sub E S Q *)
       * rewrite_env (nil ++ (F ++ Z ~ P) ++ E).
-        apply sub_weakening; simpl_env; auto.
-        -- apply wf_env_tailing with (F := F ++ Z ~ P).
-           simpl_env; auto.
+        apply sub_weakening...
+        -- apply wf_env_tailing with (F := F ++ Z ~ P)...
         -- apply wf_typ'_from_wf_typ.
-           apply wf_typ_from_bind with (F := F) (X := Z); auto.
+           apply wf_typ_from_wf_env with (F := F) (X := Z)...
         -- apply wf_typ'_from_wf_typ.
-           apply wf_typ_from_bind with (F := F) (X := Z); auto.
+           apply wf_typ_from_wf_env with (F := F) (X := Z)...
       (* sub E Q T *)
       * analyze_binds_uniq H.
-        -- apply uniq_from_wf_env; auto.
-        -- apply IHSsubT; auto.
-           ++ apply wf_typ'_from_wf_typ.
-              apply wf_typ_from_binds_typ with (X := Z); auto.
-           ++ rewrite_env (nil ++ (F ++ Z ~ P) ++ E).
-              apply wf_typ'_weakening; simpl_env.
-              ** apply wf_typ'_from_wf_typ.
-                 apply wf_typ_from_bind with (F := F) (X := Z); auto.
-              ** apply uniq_from_wf_env; auto.
-    + apply sub_var with (U := U); auto.
-      analyze_binds H.
-      apply IHSsubT; auto.
-      * apply wf_typ'_from_wf_typ.
-        apply wf_typ_from_binds_typ with (X := X); auto.
-      * apply wf_typ'_from_wf_typ.
-        apply wf_typ_from_binds_typ with (X := X); auto.
-        analyze_binds H.
-  (* NArrow *)
-  - apply sub_arrow.
-    + apply IHSsubT1; auto.
-      * inversion HwfEqT; auto.
-      * inversion HwfEqS; auto.
-      * inversion HwfEpT; auto.
-      * inversion HwfEpS; auto.
-    + apply IHSsubT2; auto.
-      * inversion HwfEqS; auto.
-      * inversion HwfEqT; auto.
-      * inversion HwfEpS; auto.
-      * inversion HwfEpT; auto.
+        apply IHSsubT...
+        -- apply wf_typ'_from_wf_typ.
+           apply wf_typ_from_binds with (X := Z)...
+        -- rewrite_env ((F ++ Z ~ P) ++ E).
+           apply wf_typ'_weaken_head...
+           apply wf_typ'_from_wf_typ.
+           apply wf_typ_from_wf_env with (F := F) (X := Z)...
+    + apply sub_var with (U := U)...
+      analyze_binds H; apply IHSsubT; eauto;
+        apply wf_typ'_from_wf_typ;
+        eapply wf_typ_from_binds...
   (* NAll *)
-  - pick fresh Y and apply sub_all; auto.
-    + apply IHSsubT; auto.
-      * inversion HwfEqT; auto.
-      * inversion HwfEqS; auto.
-      * inversion HwfEpT; auto.
-      * inversion HwfEpS; auto.
-    + rewrite_env ((Y ~ T1 ++ F) ++ Z ~ P ++ E).
-      apply H0; simpl_env; auto.
-      * apply wf_env_sub; auto.
-        inversion HwfEqT; auto.
-      * apply wf_typ'_open with (T1 := S1); eauto.
-        -- apply wf_env_sub; auto.
-           inversion HwfEqT; auto.
-        -- rewrite_env (nil ++ Y ~ T1 ++ F ++ Z ~ Q ++ E).
-           apply wf_typ'_weakening; simpl_env; auto.
-           apply uniq_from_wf_env.
-           apply wf_env_sub; auto.
-           inversion HwfEqT; auto.
-      * apply wf_typ'_open with (T1 := T1); eauto.
-        -- apply wf_env_sub; auto.
-           inversion HwfEqT; auto.
-        -- rewrite_env (nil ++ Y ~ T1 ++ F ++ Z ~ Q ++ E).
-           apply wf_typ'_weakening; simpl_env; auto.
-           apply uniq_from_wf_env.
-           apply wf_env_sub; auto.
-           inversion HwfEqT; auto.
-      * apply wf_env_sub; auto.
-        inversion HwfEpT; auto.
-      * apply wf_typ'_open with (T1 := S1); eauto.
-        -- apply wf_env_sub; auto.
-           inversion HwfEpT; auto.
-        -- rewrite_env (nil ++ Y ~ T1 ++ F ++ Z ~ P ++ E).
-           apply wf_typ'_weakening; simpl_env; auto.
-           apply uniq_from_wf_env.
-           apply wf_env_sub; auto.
-           inversion HwfEpT; auto.
-      * apply wf_typ'_open with (T1 := T1); eauto.
-        -- apply wf_env_sub; auto.
-           inversion HwfEpT; auto.
-        -- rewrite_env (nil ++ Y ~ T1 ++ F ++ Z ~ P ++ E).
-           apply wf_typ'_weakening; simpl_env; auto.
-           apply uniq_from_wf_env.
-           apply wf_env_sub; auto.
-           inversion HwfEpT; auto.
+  - pick fresh Y and apply sub_all...
+    rewrite_env ((Y ~ T1 ++ F) ++ Z ~ P ++ E).
+    apply H0; try eapply wf_typ'_open...
 Qed.
 
 Theorem sub_transitivity :
@@ -443,7 +106,7 @@ Theorem sub_transitivity :
   forall S, wf_typ' E S -> sub E S Q ->
   forall T, wf_typ' E T -> sub E Q T ->
   sub E S T.
-Proof.
+Proof with simpl_env; eauto using wf_typ'_weaken_head.
   intros E HwfE Q HwfQ.
   assert (W : type Q).
   {
@@ -456,110 +119,35 @@ Proof.
   induction W; intros Q' Heq E HwfE HwfQ S HwfS SsubQ.
   (* NTop *)
   - subst; intros T HwfT QsubT.
-    inversion QsubT; subst; auto.
+    inversion QsubT; subst...
   (* NVar *)
-  - induction SsubQ; subst; try discriminate; auto.
+  - induction SsubQ; subst; try discriminate...
     intros T HwfT QsubT.
-    apply sub_var with (U := U); auto.
-    apply IHSsubQ; auto.
+    apply sub_var with (U := U)...
+    apply IHSsubQ...
     apply wf_typ'_from_wf_typ.
-    apply wf_typ_from_binds_typ with (X := X0); auto.
+    apply wf_typ_from_binds with (X := X0)...
   (* NArrow *)
   - induction SsubQ; subst; try discriminate; intros T HwfT QsubT.
-    + inversion QsubT; subst; auto.
-      apply sub_var with (U := U); auto.
-      apply IHSsubQ; auto.
+    + inversion QsubT; subst...
+      apply sub_var with (U := U)...
+      apply IHSsubQ...
       apply wf_typ'_from_wf_typ.
-      apply wf_typ_from_binds_typ with (X := X); auto.
-    + inversion Heq; inversion QsubT; subst; auto.
-      apply sub_arrow; auto.
-      * apply IHW1 with (Q' := T1); auto.
-        -- inversion HwfQ; auto.
-        -- inversion HwfT; auto.
-        -- inversion HwfS; auto.
-      * apply IHW2 with (Q' := T2); auto.
-        -- inversion HwfQ; auto.
-        -- inversion HwfS; auto.
-        -- inversion HwfT; auto.
+      apply wf_typ_from_binds with (X := X)...
+    + inversion Heq; inversion QsubT; subst...
   (* NAll *)
   - induction SsubQ; subst; try discriminate; intros T HwfT QsubT.
-    + inversion QsubT; subst; auto.
-      apply sub_var with (U := U); auto.
-      apply IHSsubQ; auto.
+    + inversion QsubT; subst...
+      apply sub_var with (U := U)...
+      apply IHSsubQ...
       apply wf_typ'_from_wf_typ.
-      apply wf_typ_from_binds_typ with (X := X); auto.
-    + inversion Heq; inversion QsubT; subst; auto.
+      apply wf_typ_from_binds with (X := X)...
+    + inversion Heq; inversion QsubT; subst...
       pick fresh Y and apply sub_all.
-      * apply IHW with (Q' := T1); auto.
-        -- inversion HwfQ; auto.
-        -- inversion HwfT; auto.
-        -- inversion HwfS; auto.
-      * apply H0 with (X := Y) (Q' := open_tt T2 Y); auto.
-        -- apply wf_env_sub; auto.
-           inversion HwfT; auto.
-        -- apply wf_typ'_open with (T1 := T1) (U := Y); auto.
-           ++ inversion HwfT; auto.
-           ++ rewrite_env (nil ++ Y ~ T4 ++ E).
-              apply wf_typ'_weakening; auto.
-              simpl_env.
-              apply uniq_from_wf_env.
-              apply wf_env_sub; auto.
-              inversion HwfT; auto.
-           ++ apply wf_typ_var with (U := T4); auto.
-        -- apply wf_typ'_open with (T1 := S1) (U := Y); auto.
-           ++ inversion HwfT; auto.
-           ++ rewrite_env (nil ++ Y ~ T4 ++ E).
-              apply wf_typ'_weakening; auto.
-              simpl_env.
-              apply uniq_from_wf_env.
-              apply wf_env_sub; auto.
-              inversion HwfT; auto.
-           ++ apply wf_typ_var with (U := T4); auto.
-        -- rewrite_env (nil ++ Y ~ T4 ++ E).
-           apply sub_narrowing_aux with (Q := T1); simpl_env; eauto.
-           ++ apply wf_env_sub; auto.
-              inversion HwfQ; auto.
-           ++ apply wf_env_sub; auto.
-              inversion HwfT; auto.
-           ++ apply wf_typ'_open with (T1 := S1); eauto.
-              ** apply wf_env_sub; auto.
-                 inversion HwfQ; auto.
-              ** rewrite_env (nil ++ Y ~ T1 ++ E).
-                 apply wf_typ'_weakening; simpl_env; auto.
-                 apply uniq_from_wf_env; auto.
-                 apply wf_env_sub; auto.
-                 inversion HwfQ; auto.
-           ++ apply wf_typ'_open with (T1 := T1); eauto.
-              ** apply wf_env_sub; auto.
-                 inversion HwfQ; auto.
-              ** rewrite_env (nil ++ Y ~ T1 ++ E).
-                 apply wf_typ'_weakening; simpl_env; auto.
-                 apply uniq_from_wf_env; auto.
-                 apply wf_env_sub; auto.
-                 inversion HwfQ; auto.
-           ++ apply wf_typ'_open with (T1 := S1); eauto.
-              ** apply wf_env_sub; auto.
-                 inversion HwfT; auto.
-              ** rewrite_env (nil ++ Y ~ T4 ++ E).
-                 apply wf_typ'_weakening; simpl_env; auto.
-                 apply uniq_from_wf_env; auto.
-                 apply wf_env_sub; auto.
-                 inversion HwfT; auto.
-           ++ apply wf_typ'_open with (T1 := T1); eauto.
-              ** apply wf_env_sub; auto.
-                 inversion HwfT; auto.
-              ** rewrite_env (nil ++ Y ~ T4 ++ E).
-                 apply wf_typ'_weakening; simpl_env; auto.
-                 apply uniq_from_wf_env; auto.
-                 apply wf_env_sub; auto.
-                 inversion HwfT; auto.
-        -- apply wf_typ'_open with (T1 := T4) (U := Y); auto.
-           ++ inversion HwfT; auto.
-           ++ rewrite_env (nil ++ Y ~ T4 ++ E).
-              apply wf_typ'_weakening; auto.
-              simpl_env.
-              apply uniq_from_wf_env.
-              apply wf_env_sub; auto.
-              inversion HwfT; auto.
-           ++ apply wf_typ_var with (U := T4); auto.
+      * apply IHW with (Q' := T1)...
+      * apply H0 with (X := Y) (Q' := open_tt T2 Y); eauto;
+          try eapply wf_typ'_open...
+        rewrite_env (nil ++ Y ~ T4 ++ E);
+          apply sub_narrowing_aux with (Q := T1); eauto;
+          try eapply wf_typ'_open...
 Qed.
